container/coq/pointer/Layer1/Layer.v
@@ -49,7 +49,6 @@ Section Layer1_Layer.
           :: ("addr_is_level_aligned", prim addr_is_level_aligned_spec)
           :: ("atomic_add_64", prim atomic_add_64_spec)
           :: ("buffer_map", prim buffer_map_spec)
-          :: ("data_create_internal", prim data_create_internal_spec)
           :: ("find_lock_two_granules", prim find_lock_two_granules_spec)
           :: ("get_tte", prim get_tte_spec)
           :: ("granule_addr", prim granule_addr_spec)
