container/coq/pointer/Layer3/Layer.v
@@ -53,7 +53,6 @@ Section Layer3_Layer.
           :: ("addr_to_granule", prim addr_to_granule_spec)
           :: ("addr_to_idx", prim addr_to_idx_spec)
           :: ("atomic_add_64", prim atomic_add_64_spec)
-          :: ("data_create_internal", prim data_create_internal_spec)
           :: ("entry_is_table", prim entry_is_table_spec)
           :: ("find_lock_two_granules", prim find_lock_two_granules_spec)
           :: ("get_tte", prim get_tte_spec)
