container/coq/pointer/Layer5/granule_pa_to_va/LowSpec.v
@@ -11,7 +11,7 @@ Section Layer5_granule_pa_to_va_LowSpec.
   Context `{int_ptr: IntPtrCast}.
 
   Definition granule_pa_to_va_spec_low (v_0: Z) (st: RData) : (option (Ptr * RData)) :=
-    rely (((((v_0 - (MEM0_PHYS)) >= (0)) /\ (((v_0 - ((MEM0_PHYS + (MEM0_SIZE)))) < (0)))) \/ ((((v_0 - (MEM1_PHYS)) >= (0)) /\ (((v_0 - ((MEM1_PHYS + (MEM1_SIZE)))) < (0)))))));
+    rely (((((v_0 - (MEM0_PHYS)) >= (0)) /\ (((v_0 - (4294967296)) < (0)))) \/ ((((v_0 - (MEM1_PHYS)) >= (0)) /\ (((v_0 - (556198264832)) < (0)))))));
     if ((v_0 & (549755813888)) =? (0))
     then (Some ((int_to_ptr (v_0 + (18446744004990074880))), st))
     else (Some ((int_to_ptr (v_0 + (18446743457381744640))), st)).
