container/coq/pointer/Layer6/ns_buffer_read/LowSpec.v
@@ -12,16 +12,9 @@ Section Layer6_ns_buffer_read_LowSpec.
   Context `{int_ptr: IntPtrCast}.
 
   Definition ns_buffer_read_spec_low (v_0: Z) (v_1: Z) (v_2: Z) (v_3: Ptr) (st: RData) : (option (bool * RData)) :=
-    rely (((((v_1 - (MEM0_PHYS)) >= (0)) /\ (((v_1 - ((MEM0_PHYS + (MEM0_SIZE)))) < (0)))) \/ ((((v_1 - (MEM1_PHYS)) >= (0)) /\ (((v_1 - ((MEM1_PHYS + (MEM1_SIZE)))) < (0)))))));
-    if ((v_1 & (549755813888)) =? (0))
-    then (
-      rely (((((int_to_ptr (v_1 + (18446744004990074880))).(pbase)) = ("granule_data")) /\ ((((int_to_ptr (v_1 + (18446744004990074880))).(poffset)) >= (0)))));
-      when v_6, st_2 == ((memcpy_ns_read_spec_state_oracle v_3 (int_to_ptr (v_1 + (18446744004990074880))) v_2 st));
-      (Some (v_6, st_2)))
-    else (
-      rely (((((int_to_ptr (v_1 + (18446743457381744640))).(pbase)) = ("granule_data")) /\ ((((int_to_ptr (v_1 + (18446743457381744640))).(poffset)) >= (0)))));
-      when v_6, st_2 == ((memcpy_ns_read_spec_state_oracle v_3 (int_to_ptr (v_1 + (18446743457381744640))) v_2 st));
-      (Some (v_6, st_2))).
+    when v_5, st_0 == ((granule_pa_to_va_spec v_1 st));
+    when v_6, st_1 == ((memcpy_ns_read_spec v_3 v_5 v_2 st_0));
+    (Some (v_6, st_1)).
 
 End Layer6_ns_buffer_read_LowSpec.
 
