container/coq/pointer/Layer6/ns_buffer_unmap/LowSpec.v
@@ -2,7 +2,6 @@ Require Import Code.
 Require Import CommonDeps.
 Require Import DataTypes.
 Require Import GlobalDefs.
-Require Import Layer5.Spec.
 
 Local Open Scope string_scope.
 Local Open Scope Z_scope.
